code/mpfr/MPFR.Lib.Spec.fst
@@ -1,7 +1,7 @@
 module MPFR.Lib.Spec
 
 open FStar.Mul
-open MPFR.FloatingPoint
+open MPFR.Dyadic
 open MPFR.Maths
 
 #set-options "--z3refresh --z3rlimit 5 --max_fuel 1 --initial_fuel 0 --max_ifuel 1 --initial_ifuel 0"
@@ -12,9 +12,15 @@ open MPFR.Maths
 //  Used to store IEEE format floating point number  //
 ///////////////////////////////////////////////////////
 
-(* Note that 0 is not supported *)
+(* MPFR uses 'mpfr_sign', 'mpfr_prec', 'mpfr_exp' and 'mpfr_d' to describe a dyadic rational number
+ * 'mpfr_d' is an array of uint64 represent the mantissa in the following way:
+ * it should start with bit '1' and the last certain bits (depends on precision) should be '0's
+ * thus it represent a number in [0.5, 1) by adding '0.' in front of it.
+ * This struct is going to follow similar rules:
+ * 'sign', 'prec' and 'exp' give the sign, precision and exponent of the number resprectively
+ * 'limb' is a 'len'-bit natural number (possibly with leading zeros) represents the significand *)
 type fp_struct = {
-    sign: (s:int{s = -1 \/ s = 1});
+    sign: s:int{s = -1 \/ s = 1};
     prec: pos;
     exp : int;
     limb: nat;
@@ -30,28 +36,34 @@ let mk_struct sign prec exp limb len = {
 }
 
 (* Get bit length of a positive integer *)
-val bits: m:pos -> Tot (p:pos{pow2 (p - 1) <= m /\ m < pow2 p})
-let bits m = log2 m + 1
+val nb_of_bits: m:pos -> Tot (p:pos{pow2 (p - 1) <= m /\ m < pow2 p})
+let nb_of_bits m = log2 m + 1
 
-type valid_struct = s:fp_struct{s.limb = 0 \/ bits s.limb <= s.len}
+val nb_of_bits_lemma: m:pos -> p:pos{pow2 (p - 1) <= m /\ m < pow2 p} ->
+    Lemma (nb_of_bits m = p)
+let nb_of_bits_lemma m p =
+    lemma_log2_le (pow2 (p - 1)) m;
+    lemma_log2_lt m p
+
+type valid_struct = s:fp_struct{s.limb = 0 \/ nb_of_bits s.limb <= s.len}
 
 (* Evaluation. Here is the method.
  * Firstly add '0.' in front of 'limb' to make it a floating number in (0, 1)
  * Then multiply it with 2 ^ exp *)
-let eval (fp:fp_struct) = mk_fp (fp.sign * fp.limb) (fp.exp - fp.len)
+let eval (fp:valid_struct) = mk_fp (fp.sign * fp.limb) (fp.exp - fp.len)
 
 
 /////////////////////////////////////////////////////////////////////////////////////////
 //  Validity Test for ieee_struct                                                      //
 //  A valid struct represents a binary floating point number defined in MPFR.BinaryFP  //
-//  Important function 'eval' maps ieee_fp to floating_point                                //
+//  Important function 'eval' maps ieee_fp to dyadic                                   //
 /////////////////////////////////////////////////////////////////////////////////////////
 
 (* Condition for validity 
  * A valid struct should have a positive precision which is smaller than 'limb' length
  * Only the first 'prec' bits of 'limb' store value and the rest bits are 0s *)
 let ieee_valid_cond (s:fp_struct) =
-    s.limb > 0 /\ bits s.limb = s.len /\
+    s.limb > 0 /\ nb_of_bits s.limb = s.len /\
     0 < s.prec /\ s.prec <= s.len /\
     s.limb % pow2 (s.len - s.prec) = 0
     
@@ -72,7 +84,7 @@ let mk_ieee sign prec exp limb len: Pure ieee_fp
 let gmp_NUMB_BITS = 64
 let mpfr_PREC_MIN = 1
 let mpfr_PREC_MAX = pow2 31 - 1
-let mpfr_PREC_COND (p:pos) = mpfr_PREC_MIN <= p /\ p <= mpfr_PREC_MAX
+let mpfr_PREC_COND (p:nat) = mpfr_PREC_MIN <= p /\ p <= mpfr_PREC_MAX
 
 let mpfr_EXP_INVALID = pow2 30
 let mpfr_EMIN = 1 - mpfr_EXP_INVALID
@@ -85,6 +97,17 @@ let mpfr_EXP_COND (x:int) = mpfr_EMIN <= x /\ x <= mpfr_EMAX
 val arr_size: p:pos ->
     Tot (s:pos{s % 64 = 0 /\ s >= p /\ s - 64 < p})
 let arr_size p = ((p + 63) / 64) * 64
+
+val arr_size_lemma: p:pos -> s:pos{s % 64 = 0 /\ s >= p /\ s - 64 < p} ->
+    Lemma (arr_size p = s)
+let arr_size_lemma p s =
+    lemma_div_le (p + 63) (s + 63) 64;
+    //lemma_div_distr s 63 64;
+    //! assert((p + 63) / 64 <= s);
+    lemma_div_le s (p + 63) 64;
+    //lemma_multiple_div s 64;
+    //! assert(s <= (p + 63) / 64);
+    ()
 
 let mpfr_valid_cond (s:ieee_fp) =
     s.len = arr_size s.prec /\
